hoare

hoare/Semantics.v
@@ -1,8 +1,10 @@
 Require Import String.
 Require Import List.
 Import ListNotations.
-Require Import syntax.
+Require Import Syntax.
 Require Import util.
+
+Arguments Env dom codom : clear implicits.
 
 Instance AddrTEq : EqDec AddrT.
     constructor.
@@ -17,8 +19,6 @@ Variant UndefVal :=
     | Undef
     | Defined (v:Val).
 
-
-
 Notation VarEnv := (Env VarT AddrT).
 Notation MemEnv := (Env AddrT UndefVal).
 
@@ -27,12 +27,12 @@ Notation MemEnv := (Env AddrT UndefVal).
         var_assign: VarEnv;
         memory_assign: MemEnv
     }. *)
-Definition State := (list VarEnv * MemEnv)%type.
+Definition State := (VarEnv * MemEnv)%type.
 
 Implicit Type (ρ:VarEnv) (ρs:list VarEnv) (μ:MemEnv) (σ:State).
 
 
-Definition ρmap σ := lookupStack (fst σ).
+Definition ρmap σ := lookup (fst σ).
 Definition μmap σ := lookup (snd σ).
 
 Definition lookupVar σ x :=
@@ -46,21 +46,22 @@ Definition evalOp (op:Op) (v1 v2:Val) : option Val :=
     | Mul, IntVal i1, IntVal i2 => Some (IntVal (i1*i2))
     | Ge , IntVal i1, IntVal i2 => Some (IntVal (if Nat.leb i2 i1 then 1 else 0))
     | Eq , IntVal i1, IntVal i2 => Some (IntVal (if Nat.eqb i1 i2 then 1 else 0))
+    | And, IntVal i1, IntVal i2 => Some (IntVal (if Nat.eqb 0 i1 then 0 else i2))
+    | Lt , IntVal i1, IntVal i2 => Some (IntVal (if Nat.ltb i1 i2 then 1 else 0))
     | _, _, _ => None
     end.
 
-Fixpoint LExprEval (l:LExpr) (σ:State) : option AddrT :=
+Definition evalUOp (uop:UOp) (v1:Val) : option Val :=
+    match uop, v1 with 
+    | Not, IntVal i1 => Some (IntVal (if Nat.eqb 0 i1 then 1 else 0))
+    | _, _ => None
+    end.
+
+Definition LExprEval (l:LExpr) (σ:State) : option AddrT :=
     match l with
-    (* C0b *)
     | Var x => ρmap σ x
-    (* C0p *)
-    | Indir e => 
-        match RExprEval e σ with
-        | Some (AddrVal a) => Some a
-        | _ => None
-        end
-    end
-with RExprEval (e:Expr) (σ:State) : option Val :=
+    end.
+Fixpoint RExprEval (e:Expr) (σ:State) : option Val :=
     match e with 
     | Const c => ret c
     | LVal l => 
@@ -75,12 +76,9 @@ with RExprEval (e:Expr) (σ:State) : option Val :=
         v1 <- RExprEval e1 σ;;
         v2 <- RExprEval e2 σ;;
         evalOp op v1 v2
-    (* C0p *)
-    | Addr e => 
-        match LExprEval e σ with
-        | Some a => Some (AddrVal a)
-        | _ => None
-        end
+    | Unary op e1 =>
+        v1 <- RExprEval e1 σ;;
+        evalUOp op v1
     end
     .
 
@@ -104,40 +102,16 @@ Definition bool_to_nat (b:bool) :=
 Coercion bool_to_nat : bool >-> nat.
 Coercion IntVal : nat >-> Val.
 Coercion Defined : Val >-> UndefVal.
-(* Coercion Some : UndefVal >-> (option UndefVal). *)
 
-Definition remove_codom {A B C} {BEq:EqDec B} (μ:Env B C) (ρ:Env A B) : Env B C :=
-    undef μ (getCodom ρ).
-
-Definition maxAddr μ :=
-    list_max(map (fun a =>
-        match a with
-        | NatAddr n => n
-        | _ => 0
-        end
-    ) (getDom μ)).
-
-Definition initAdresses μ xs v :=
-    fold_left
-    (fun e a =>
-        update e a v
-    ) xs μ.
-
-Definition getNewAdresses (decl:list Declaration) μ : VarEnv :=
-    let freshAddr := S(maxAddr μ) in
-    fold_left_i (fun e '(t,v) i =>
-        let a := NatAddr (i + freshAddr) in
-        e { v ↦ a }
-    ) decl emptyEnv.
-
+Definition diverge := While (Const 1) (Block []).
 
 Reserved Notation "c1 ~> c2" (at level 50).
 Inductive step : Conf -> Conf -> Prop :=
-    | AssignStep l e ρs μ a v: 
-        let σ := (ρs, μ) in
+    | AssignStep l e ρ μ a v: 
+        let σ := (ρ, μ) in
         R⟦e⟧σ = Some v ->
         L⟦l⟧σ = Some a ->
-        ⟨ (Assign l e) | σ ⟩ ~> «(ρs, update μ a (Defined v))»
+        ⟨ (Assign l e) | σ ⟩ ~> «(ρ, update μ a (Defined v))»
     | IfTrueStep e s1 s2 σ (n:nat) :
         R⟦e⟧σ = Some (n:Val) ->
         n <> 0 ->
@@ -146,34 +120,24 @@ Inductive step : Conf -> Conf -> Prop :=
         R⟦e⟧σ = Some (0:Val) ->
         ⟨ (If e s1 s2) | σ ⟩ ~> ⟨ s2 | σ ⟩
     | WhileStep e s σ :
-        ⟨ (While e s) | σ ⟩ ~> ⟨ If e (Block [] [s; While e s]) (Block [] []) | σ ⟩
-    (* modified by C0b *)
+        ⟨ (While e s) | σ ⟩ ~> ⟨ If e (Block [s; While e s]) (Block []) | σ ⟩
     | EmptyStep σ :
-        (* or ignore decls *)
-        ⟨ Block [] [] | σ ⟩ ~> « σ »
+        ⟨ Block [] | σ ⟩ ~> « σ »
     | ExecStep s1 sr σ σ' :
         ⟨ s1 | σ ⟩ ~> « σ' » ->
-        (* or ignore decls *)
-        ⟨ Block [] (s1::sr) | σ ⟩ ~> ⟨ Block [] sr | σ' ⟩
+        ⟨ Block (s1::sr) | σ ⟩ ~> ⟨ Block sr | σ' ⟩
     | SubstStep s1 s1' sr σ σ' :
         ⟨ s1 | σ ⟩ ~> ⟨ s1' | σ' ⟩ ->
-        (* or ignore decls *)
-        ⟨ Block [] (s1::sr) | σ ⟩ ~> ⟨ Block [] (s1'::sr) | σ' ⟩
+        ⟨ Block (s1::sr) | σ ⟩ ~> ⟨ Block (s1'::sr) | σ' ⟩
     | AbortStep σ :
         ⟨ Abort | σ ⟩ ~> ↯
     | CrashStep s1 sr σ :
         ⟨ s1 | σ ⟩ ~> ↯ ->
-        (* or ignore decls *)
-        ⟨ Block [] (s1::sr) | σ ⟩ ~> ↯
-    (* added by C0b *)
-    | BlockStep decl stmt ρs μ:
-        let ρ := getNewAdresses decl μ in
-        let addrs := getCodom ρ in
-        ⟨ Block decl stmt | (ρs,μ) ⟩ ~> 
-        ⟨ Block [] (stmt++[■]) | (ρ::ρs, initAdresses μ addrs Undef) ⟩
-    | LeaveStep ρ ρs μ:
-        ⟨ Block [] [■] | (ρ::ρs, μ) ⟩  ~>
-        « (ρs,remove_codom μ ρ) »
+        ⟨ Block (s1::sr) | σ ⟩ ~> ↯
+    | AssertStep e σ:
+        ⟨ Assert e | σ ⟩ ~> ⟨ If e (Block []) (Abort) | σ ⟩
+    | AssumeStep e σ:
+        ⟨ Assume e | σ ⟩ ~> ⟨ If e (Block []) (diverge) | σ ⟩
     where "c1 ~> c2" := (step c1 c2).
 
 Inductive trace : list Conf -> Prop :=
