hoare/Hoare.v
@@ -1,0 +1,293 @@
+Require Import Syntax.
+Require Import Semantics.
+Require Import util.
+Require Import List.
+Import ListNotations.
+
+Instance LExprEq : EqDec LExpr.
+    constructor.
+    now repeat decide equality.
+Defined.
+
+
+Lemma terminalTerminated :
+    forall (σ:State),
+    terminal (Terminated σ).
+Proof.
+    intros.
+    intros [c' H].
+    inversion H.
+Qed.
+
+Lemma terminalAbortion :
+    terminal ↯.
+Proof.
+    intros.
+    intros [c' H].
+    inversion H.
+Qed.
+
+
+
+
+
+
+Section Syntactic.
+
+    Definition Property := Expr.
+
+    Implicit Type (P Q:Property) (e:Expr) (s:Stmt) (x:LExpr).
+
+    Fixpoint replace P e x {struct P} :=
+        match P with
+        | Binary o e1 e2 => Binary o (replace e1 e x) (replace e2 P x)
+        | LVal l => if eqdec l x then e else P
+        | _ => P
+        end.
+
+    Definition interpret P σ :=
+        exists n, RExprEval P σ = Some (IntVal n) /\ n<>0.
+    Notation "P ⟦ σ ⟧ " := (interpret P σ) (at level 70).
+    Notation "P ⇒ Q" := (forall σ, P⟦σ⟧ -> Q⟦σ⟧) (at level 60).
+    (* Notation "P ⟦ E ⌿ x ⟧" := (replace P E x) (at level 50). *)
+
+    Reserved Notation "{{ P }} s {{ Q }}" (at level 50).
+    Inductive hoare : Property -> Stmt -> Property -> Prop :=
+        | hoareConsequence P P' s Q Q':
+            (P ⇒ P') ->
+            (Q' ⇒ Q) ->
+            {{P'}} s {{Q'}} ->
+            {{P}} s {{Q}}
+        | hoareAssign P x e: 
+            {{ replace P e x }} (Assign x e) {{P}}
+        | hoareWhile e s P Q:
+            {{Binary And P e}} s {{P}} ->
+            {{P}} While e s {{Binary And P (Unary Not e)}}
+        | hoareIf b s1 s2 P Q:
+            {{Binary And P b}} s1 {{Q}} ->
+            {{Binary And P (Unary Not b)}} s2 {{Q}} ->
+            {{P}} If b s1 s2 {{Q}}
+        | hoareSkip P P:
+            {{P}} Block [] {{P}}
+        | hoareBlock s B P Q R:
+            {{P}} s {{Q}} ->
+            {{Q}} Block B {{R}} ->
+            {{P}} Block (s::B) {{R}}
+        | hoareAssert P e:
+            (P ⇒ e) ->
+            {{P}} (Assert e) {{P}}
+        | hoareAssume P e:
+            {{P}} (Assume e) {{Binary And P e}}
+        where "{{ P }} s {{ Q }}" := (hoare P s Q).
+
+    Ltac inv_subst H :=
+        inversion H;subst;clear H.
+
+    Lemma bigstep_terminal_inv σ σ':
+    « σ » ⇓ « σ' » -> σ = σ'.
+    Proof.
+        intros H.
+        inv_subst H.
+        - reflexivity.
+        - inversion H0.
+    Qed.
+
+    Lemma And_split P Q σ:
+        P ⟦ σ ⟧ ->
+        Q ⟦ σ ⟧ ->
+        Binary And P Q ⟦ σ ⟧.
+    Proof.
+        intros [n [HP Hn]] [m [HQ Hm]].
+        exists m;split;[|assumption];cbn.
+        rewrite HP, HQ;cbn.
+        destruct n;congruence.
+    Qed.
+
+    Scheme dep_elim_hoare := Induction for hoare Sort Prop.
+    Scheme dep_elim_bigStep := Induction for bigStep Sort Prop.
+
+    From Equations Require Import Equations.
+    Derive Signature for bigStep.
+    Derive Signature for step.
+
+    Lemma abort_not_terminate σ:
+        ~ ↯ ⇓ « σ ».
+    Proof.
+        intros H.
+        inv_subst H.
+        inversion H0.
+    Qed.
+
+    Derive NoConfusion for Conf.
+    Derive NoConfusion for Stmt.
+
+    (* define alternative bigstep semantic for easier proofs *)
+
+    Lemma diverge_not_terminate σ σ':
+        ~ ⟨ diverge | σ ⟩ ⇓ « σ' ».
+    Proof.
+    (* needs dep elim *)
+    Admitted.
+
+    Lemma bigstep_block_inv s B σ σ'':
+     ⟨ Block (s::B) | σ ⟩ ⇓ « σ'' » ->
+     exists σ', ⟨ s | σ ⟩ ⇓ « σ' » /\ 
+        ⟨ Block B | σ' ⟩ ⇓ « σ'' ».
+    Proof.
+        intros H.
+        inv_subst H.
+        inv_subst H0. (* needs dep_elim *)
+        - exists σ';split.
+          + econstructor.
+            eassumption.
+            constructor.
+            apply terminalTerminated.
+          + assumption.
+        - (* needs dep_elim *)
+          admit.
+        - apply abort_not_terminate in H1.
+          contradict H1.
+    Admitted.
+
+    Lemma Not_expr e σ:
+        R⟦ e ⟧ σ = Some (IntVal 0) ->
+        Unary Not e ⟦ σ ⟧.
+    Proof.
+        intros H.
+        exists 1;split;[|auto].
+        cbn.
+        rewrite H.
+        cbn. reflexivity.
+    Qed.
+
+
+    Lemma partial_correctness P Q s:
+        hoare P s Q ->
+        forall σ, (P⟦σ⟧) ->
+        forall σ', ⟨ s | σ ⟩ ⇓ « σ' » ->
+        (Q⟦σ'⟧).
+    Proof.
+        induction 1;intros σ HP σ' HTerm.
+        - enough (Q' ⟦ σ' ⟧).
+          {
+            now apply H0.
+          }
+          eapply IHhoare.
+          1: apply (H σ HP).
+          apply HTerm.
+        - inv_subst HTerm.
+          inv_subst H. subst σ0.
+          apply bigstep_terminal_inv in H0 as <-.
+          unfold interpret in *.
+          induction P;destruct HP as [n [He Hn]].
+          + exists n. now split.
+          + admit.
+          + admit.
+          + unfold replace in He.
+            destruct (eqdec l x) as [<-|].
+            * assert(v=IntVal n) as ->.
+              {
+                enough (Some v = Some (IntVal n)) by now inv_subst H.
+                rewrite <- H5, <- He.
+                induction e;admit.
+              }
+              exists n.
+              split.
+              2: assumption.
+              cbn.
+              assert(L⟦l⟧ (ρ,μ {a↦n}) = L⟦l⟧ (ρ,μ)) as -> by admit.
+              rewrite H6.
+              unfold μmap.
+              cbn.
+              assert(lookup (μ {a ↦ n}) a = Some (Defined (IntVal n))) as -> by admit.
+              reflexivity.
+            * exists n.
+              cbn in He.
+              assert(exists b, L⟦ l ⟧ (ρ,μ) = Some b) as [b Hb].
+              {
+                destruct (L⟦ l ⟧ (ρ,μ)).
+                - now exists a0.
+                - inversion He.
+              }
+              cbn.
+              admit.
+              (* assert(L⟦l⟧ (ρ,μ {a↦v}) = L⟦l⟧ (ρ,μ)) as -> by admit.
+              rewrite Hb.
+              unfold μmap.
+              cbn.
+              assert(lookup (μ {a ↦ n}) a = Some (Defined (IntVal n))) as -> by admit. *)
+        - inv_subst HTerm.
+          inv_subst H0.
+          inv_subst H1.
+          inv_subst H0.
+          + apply bigstep_block_inv in H2 as [σ'' [Hs HB]].
+            apply And_split.
+            * admit. (* needs dep elim *)
+            * admit. (* after while false *)
+          + inv_subst H2.
+            inv_subst H0.
+            apply bigstep_terminal_inv in H1 as <-.
+            apply And_split.
+            * assumption.
+            * now apply Not_expr.
+        - inv_subst HTerm.
+          inv_subst H1.
+          + eapply IHhoare1.
+            2: eassumption.
+            apply And_split.
+            * assumption.
+            * exists n;split;auto.
+          + eapply IHhoare2.
+            2: eassumption.
+            apply And_split.
+            * assumption.
+            * now apply Not_expr.
+        - inv_subst HTerm.
+          inv_subst H.
+          apply bigstep_terminal_inv in H0 as <-.
+          assumption.
+        - apply bigstep_block_inv in HTerm as [σ'' [Hs HB]].
+          eapply IHhoare2.
+          2: eassumption.
+          eapply IHhoare1.
+          1: apply HP.
+          assumption.
+        - inv_subst HTerm.
+          inv_subst H0.
+          inv_subst H1.
+          inv_subst H0.
+          + inv_subst H2.
+            inv_subst H0.
+            apply bigstep_terminal_inv in H1 as <-.
+            assumption.
+          + inv_subst H2.
+            inv_subst H0.
+            inv_subst H1.
+            inversion H0.
+        - inv_subst HTerm.
+          inv_subst H.
+          inv_subst H0.
+          inv_subst H.
+          + inv_subst H1.
+            inv_subst H.
+            apply bigstep_terminal_inv in H0 as <-.
+            apply And_split.
+            * assumption.
+            * exists n;split;assumption.
+          + apply diverge_not_terminate in H1.
+            contradict H1.
+    Qed.
+
+
+
+
+    (* while with termination proof *)
+    (* Lemma total_correctness P Q s σ:
+        hoare P s Q ->
+        P σ ->
+        exists σ',
+        ⟨ s | σ ⟩ ⇓ « σ' » /\
+        Q σ'.
+    Proof. *)
+
+End Syntactic.
