hoare/Syntax.v
@@ -1,0 +1,56 @@
+Require Import String.
+Require Import List.
+Require Import Nat.
+Import ListNotations.
+
+Definition VarT := string.
+(* Definition Addr := nat. *)
+Variant AddrT := Triangle | Circle | Pentagon | Square | NatAddr (n:nat).
+Variant Val :=
+    | AddrVal (addr: AddrT)
+    | IntVal (v: nat).
+
+
+Variant Op := 
+    Lt | Eq | Add | Mul | Sub | And | Ge.
+     (* | Ge | Eq |
+    And | Xor. *)
+(* define Ge with Lt & Eq & Not *)
+    (* Lt Eq *)
+Variant UOp := Not.
+
+(* Variant BinaryNotationOp :=
+    And | Ge | Xor.
+Variant UnaryNotationOp :=
+    Not. *)
+
+Inductive Expr :=
+    | Const (c:Val)
+    | Binary (o:Op) (e1 e2:Expr)
+    | Unary (o:UOp) (e1:Expr)
+    | LVal (l:LExpr)
+with LExpr :=
+    | Var (v:VarT)
+    .
+
+Implicit Type (e : Expr) (c : Val) (x y : VarT).
+
+Inductive Stmt :=
+    | Assume e
+    | Assert e
+    | While e (s:Stmt)
+    | If e (s_then s_else : Stmt)
+    | Block (h:list Stmt)
+    | Assign (x:LExpr) e
+    | Abort
+    .
+
+Implicit Type (ss : list Stmt) (s:Stmt).
+
+
+
+
+Notation "△" := Triangle.
+Notation "○" := Circle.
+Notation "⬠" := Pentagon.
+Notation "□" := Square.
